crypto.v
@@ -795,22 +795,20 @@ Proof. by iIntros "? ?"; rewrite pterm_TEnc; eauto. Qed.
 
 Section TermMeta.
 
-Context `{Countable L}.
-
 Class TermMeta
-  (term_meta : term → namespace → L → iProp)
+  (term_meta : ∀ `{Countable L}, term → namespace → L → iProp)
   (term_meta_token : term → coPset → iProp) := {
-  term_meta_timeless :> ∀ t N (x : L),
+  term_meta_timeless :> ∀ `{Countable L} t N (x : L),
     Timeless (term_meta t N x);
-  term_meta_persistent :> ∀ t N (x : L),
+  term_meta_persistent :> ∀ `{Countable L} t N (x : L),
     Persistent (term_meta t N x);
-  term_meta_set : ∀ E t (x : L) N,
+  term_meta_set : ∀ `{Countable L} E t (x : L) N,
     ↑N ⊆ E →
     term_meta_token t E ==∗ term_meta t N x;
-  term_meta_meta_token : ∀ t (x : L) N E,
+  term_meta_meta_token : ∀ `{Countable L} t (x : L) N E,
     ↑N ⊆ E →
     term_meta_token t E -∗ term_meta t N x -∗ False;
-  term_meta_agree : ∀ t N (x1 x2 : L),
+  term_meta_agree : ∀ `{Countable L} t N (x1 x2 : L),
     term_meta t N x1 -∗
     term_meta t N x2 -∗
     ⌜x1 = x2⌝;
@@ -822,7 +820,7 @@ Class TermMeta
 
 (* Using two locations is a bit ugly, but maybe more convenient *)
 
-Definition nonce_meta t N (x : L) : iProp :=
+Definition nonce_meta `{Countable L} t N (x : L) : iProp :=
   match t with
   | TNonce a => ∃ a', meta a (nroot.@"meta") a' ∧ meta a' N x
   | _ => False
@@ -835,21 +833,21 @@ Definition nonce_meta_token t E : iProp :=
   end.
 
 Program Global Instance nonce_term_meta :
-  TermMeta nonce_meta nonce_meta_token.
+  TermMeta (@nonce_meta) nonce_meta_token.
 
-Next Obligation. case=> *; apply _. Qed.
+Next Obligation. move=> ???; case=> *; apply _. Qed.
 
-Next Obligation. case=> *; apply _. Qed.
+Next Obligation. move=> ???; case=> *; apply _. Qed.
 
 Next Obligation.
-move=> E t x N; case: t; try by move=> *; iStartProof.
+move=> ??? E t x N; case: t; try by move=> *; iStartProof.
 move=> a; iIntros (sub) "token"; rewrite /=.
 iDestruct "token" as (a') "[meta_a' token]".
 by iMod (meta_set E _ x with "token") as "meta"; eauto.
 Qed.
 
 Next Obligation.
-case; try by move=> *; iStartProof.
+move=> ???; case; try by move=> *; iStartProof.
 move=> a x N E sub /=; iIntros "token meta".
 iDestruct "token" as (a1) "[meta_a1 token]".
 iDestruct "meta"  as (a2) "[meta_a2 meta]".
@@ -858,7 +856,7 @@ by iDestruct (meta_meta_token with "token meta") as "[]".
 Qed.
 
 Next Obligation.
-case; try by move=> *; iStartProof.
+move=> ???; case; try by move=> *; iStartProof.
 move=> a * /=; iIntros "meta1 meta2".
 iDestruct "meta1" as (a1) "[meta_a1 meta1]".
 iDestruct "meta2" as (a2) "[meta_a2 meta2]".
@@ -891,7 +889,7 @@ Arguments crypto_hash_name {Σ _}.
 Arguments hash_pred {Σ _ _}.
 Arguments crypto_key_name {Σ _}.
 Arguments key_pred {Σ _ _}.
-Arguments term_meta_set {Σ _ _ _ _ } E t x N.
-Arguments term_meta_token_difference {Σ _ _ _ _} t E1 E2.
+Arguments term_meta_set {Σ _ _ _ _ _ _} E t x N.
+Arguments term_meta_token_difference {Σ _ _ _} t E1 E2.
 Arguments nonce_term_meta Σ {_}.
-Arguments TermMeta : clear implicits.
+Arguments TermMeta Σ term_meta term_meta_token : assert.
